\documentclass[a4paper, 11pt]{book}
\usepackage{comment} % enables the use of multi-line comments (\ifx \fi) 
\usepackage{lipsum} %This package just generates Lorem Ipsum filler text. 
\usepackage{fullpage} % changes the margin
\usepackage[a4paper, total={7in, 10in}]{geometry}

%\usepackage{tgadventor} % The font for the entire document can be changed here
%\usepackage{courier}
%\usepackage{charter}
\usepackage{tgcursor}

\usepackage{mathrsfs} 
\usepackage{quiver} 
\newtheorem{corollary}{Corollary}
\usepackage{graphicx}
\usepackage{tikz}

\usetikzlibrary{arrows}
\usepackage{verbatim}
\usepackage[numbered]{mcode}
\usepackage{float}
\usepackage{tikz}
    \usetikzlibrary{shapes,arrows}
    \usetikzlibrary{arrows,calc,positioning}

    \tikzset{
        block/.style = {draw, rectangle,
            minimum height=1cm,
            minimum width=1.5cm},
        input/.style = {coordinate,node distance=1cm},
        output/.style = {coordinate,node distance=4cm},
        arrow/.style={draw, -latex,node distance=2cm},
        pinstyle/.style = {pin edge={latex-, black,node distance=2cm}},
        sum/.style = {draw, circle, node distance=1cm},
    }
\usepackage{xcolor}
\usepackage{mdframed}
\usepackage[shortlabels]{enumitem}
\usepackage{indentfirst}
\usepackage{hyperref}
\usepackage{amsmath,amsfonts,amsthm, amssymb}
\usepackage{array}
\usepackage[all,textures]{xy}
\usepackage{graphicx}
\usepackage{alltt}
\usepackage{listings}
\usepackage{float}
\usepackage{tabu}
\usepackage{longtable}


\theoremstyle{plain}
\newtheorem{theorem}{Proposition}[section]
\newtheorem{proposition}[theorem]{Proposition}

\newtheorem{question}[theorem]{Question}
\newtheorem{exercise}{Exercise}[chapter]
\newtheorem{problem}[theorem]{Problem}
    
\renewcommand{\thesubsection}{\thesection.\alph{subsection}}


% Define solution environment

%%%%%%%%%%%%%%%%%%%%%%%%%%%%%%%%%%%%%%%%%%%%%%%%%%%%%%%%%%%%%%%%%%%%%%%%%%%%%%%%%%%%%%%%%%%%%%%%%%%%%%%%%%%%%%%%%%%%%%%%%%%%%%%%%%%%%%%% Original packages, custom environments, and custom commands below
  \usepackage{amsmath,amsfonts,amsthm, amssymb}
  \usepackage{fullpage}
  \usepackage{array}
  \usepackage[all,textures]{xy}
  \usepackage{graphicx}
  \usepackage{alltt}
  \usepackage{listings}
  \usepackage{float}
  \usepackage{tabu}
  \usepackage{longtable}
  \usepackage{lipsum}
  \usepackage[T1]{fontenc}
  
  \theoremstyle{plain}
  \newtheorem{innercustomgeneric}{\customgenericname}
\providecommand{\customgenericname}{}
\newcommand{\newcustomtheorem}[2]{%
  \newenvironment{#1}[1]
  {%
   \renewcommand\customgenericname{#2}%
   \renewcommand\theinnercustomgeneric{##1}%
   \innercustomgeneric
  }
  {\endinnercustomgeneric}
}

\newcustomtheorem{definition}{Definition}
\newcustomtheorem{lemma}{Lemma}

\newcommand{\mb}{\mathbf}
\newcommand{\arr}{\rightarrow}
\newcommand{\mc}{\mathcal}
\newcommand{\ms}{\mathscr}
\newcommand{\co}{\text{co}}
\newcommand{\N}{\mathbb{N}}
\newcommand{\Z}{\mathbb{Z}}
\newcommand{\R}{\mathbb{R}}
\newcommand{\la}{\langle}
\newcommand{\ra}{\rangle}
\newcommand{\op}{\oplus}
\newcommand{\od}{\odot}
\newcommand{\p}{\prime}
\newcommand{\ep}{\epsilon}
\newcommand{\hyp}{{}^*}
\newcommand{\dom}{\text{dom }}

  \setlength{\parindent}{0pt}
 
 
 \newtheorem{thm}{Exercise}
\begin{document}
  \begin{titlepage}
	\centering % Center everything on the title page
	\scshape % Use small caps for all text on the title page
	\vspace*{1.5\baselineskip} % White space at the top of the page
% ===================
%	Title Section 	
% ===================

	\rule{13cm}{1.6pt}\vspace*{-\baselineskip}\vspace*{2pt} % Thick horizontal rule
	\rule{13cm}{0.4pt} % Thin horizontal rule
	
		\vspace{0.75\baselineskip} % Whitespace above the title
% ========== Title ===============	
	{	\Huge Lectures on Hyperreals\\ 
			\vspace{4mm}
		Book by Robert Goldblatt \\	}
% ======================================
		\vspace{0.75\baselineskip} % Whitespace below the title
	\rule{13cm}{0.4pt}\vspace*{-\baselineskip}\vspace{3.2pt} % Thin horizontal rule
	\rule{13cm}{1.6pt} % Thick horizontal rule
	
		\vspace{1.75\baselineskip} % Whitespace after the title block
% =================
%	Information	
% =================
	{\large : 
		\vspace*{1.2\baselineskip}
	} \\
	\vfill

\end{titlepage}
%%%%%%%%%%%%%%%%%%%%%%%%%%%%%%%%%%%%%%%%%%%%%%%%%%%%%%%%%%%
\begingroup
\let\cleardoublepage\clearpage
\tableofcontents
\endgroup

\chapter{What are Hypereals?}

\newpage

\chapter{Large sets}

  \begin{exercise}
    If $\emptyset \not = A \subseteq I$, there is an ultrafilter $\mc{F}$ on $I$ with $A \in \mc{F}$.
  \end{exercise}
  \begin{proof}
    Define $\mc{H}=\{B \in \mathscr{P}(I): A \subseteq B\}$. Since $A$ is non empty, it follows that $\mc{H}$ has fip. Clearly, $A \in \mc{H}$, and so $A \in \mc{F}^\mc{H}$. Therefore, by zorn lemma, we know that there exists ultrafilter, $\mc{F}$, such that $A \in \mc{F}^\mc{H} \subseteq \mc{F}$.
  \end{proof}

  \begin{exercise}
    There exists a nonprincipal ultrafilter on $\N$ containing the set of even numbers, and another containing the set of odd numbers.
  \end{exercise}
  \begin{proof}
    Define $I=\{x \in \N: x=2n$ for some $n \in \N\}$. Since $I$ is infinite, we know that $\mc{F}^\co$ is proper and thus, have fip. Applying the zorn's lemma, we see that there exists ultrafilter $\mc{F}$ such that $\mc{F} \subseteq \mc{F}^\co$. However, for any $i \in I$, we have $I-\{i\} \in \mc{F}^\co \subseteq \mc{F}$ but, since $\mc{F}$ is ultrafilter, $\{i\} \in \mc{F}$. However, clearly $\{i\} \in \mc{F}^i$. Therefore, $F \not = F^i$ for any $i \in I$. Likewise we could argue about set of odd numbers.
  \end{proof}

  \begin{exercise}
    An ultrafilter on finite set must be principal.
  \end{exercise}
  \begin{proof}
    Let the set be $A=\{a_1,a_2,\cdots, a_n\}$ and $\mc{F}$ be ultrafilter on it. Since $\{a_1\} \cup \{a_2\}\cup \cdots \cup \{a_n\}=A \in \mc{F}$, it must be the case that $a_i \in \mc{F}$ for some $i$ such that $1 \leq i \leq n$. Since $\mc{F}$ is proper, for any $B \in \mc{F}$, we have $B \cap \{a_i\} \not = \emptyset$, but that means $\mc{F}=\mc{F}^{a_i}$.
  \end{proof}

  \begin{exercise}
    For $\mc{H} \subseteq \ms{P}(I)$. \\
      (i) Show that $\mc{F}^\mc{H}$ is a filter that includes $\mc{H}$, i.e. $\mc{H} \subseteq \mc{F}^\mc{H}$. \\
      (ii) Show that $\mc{F}^\mc{H}$ is included in any other filter that includes $\mc{H}$.
  \end{exercise}
  \begin{proof} $ $ \\
    (i) By the definition.\\
    (ii) Let $\mc{F}$ be a filter such that $H \subseteq \mc{F}$. Let $A \in \mc{F}^\mc{H}$, then $B_1 \cap B_2 \cap \cdots \cap B_n \subseteq A$ for some $B_1,\cdots, B_n \in \mc{H}$. Clearly, $B_1 \cap \cdots \cap B_n \in F$ and so is $A \in F$.
  \end{proof}

  \begin{exercise}
    Let $\mc{F}$ be a proper filter on $I$. \\
    (I) Show that $\mc{F} \cup \{A^c\}$ has fip iff $A \notin \mc{F}$. \\
    (II) Use (I) to deduce that $\mc{F}$ is an ultrafilter iff it is maximal proper filter on $I$.
  \end{exercise}
  \begin{proof} $ $ \\
    (I) First we prove forward implication. Notice that if $A \in \mc{F}$ then since $A \cap A^c=\emptyset$, it follows $\mc{F} \cup \{A^c\}$ does not have fip. \\
    We prove the converse implication. Notice that since $F$ is a proper filter, ie it does not contain $\emptyset$, the only way for $\mc{F} \cup \{A^c\}$ to not have fip would be $A \in \mc{F}$. \\\\

    (II) We prove the foward implication. Suppose $\mc{F}$ is an ultrafilter. Applying Zorn's lemma on proper filter $\mc{F}$, we see that there exists a maximal proper filter, $K$, such that $\mc{F} \subseteq K$. If $K \not = F$, it would mean there is some $A \in K$ such that $A \not \in \mc{F}$ but then that would mean $A^C \in \mc{F}$, and so $A^c \in K$ which contradicts the fact that $K$ is proper since it fails to satisfy fip. Therefore, we must have $F=K$. \\

    We prove the converse implication. Suppose $\mc{F}$ is maximal proper filter. For the sake of contradiction assume $\mc{F}$ is not an ultra filter i.e. there exists some $A \in \ms{P}(I)$ such that both $A, A^c \notin F$. Clearly, either $\mc{F} \cup \{A\}$ has fip or $\mc{F} \cup \{A^c\}$ does. Wlog assume $\mc{F} \cup \{A\}$ has fip. Applying Zorn's lemma on $\mc{F} \cup \{A\}$, we see that there is maximal proper filter $K$ such that $\mc{F} \cup \{A\} \subseteq K$. However this means that $\mc{F}$ is not maximal proper filter since $F \subsetneqq F \cup \{A\} \subset P(I)$.
  \end{proof}

\chapter{Ultrapower Construction of the hyperreals}

  \begin{exercise}
    (section 3.3, I). $\equiv$ is an equivalence relation on $\R^\N$.
  \end{exercise}
  \begin{proof} Let $\langle a_n \rangle, \langle b_n \rangle, \langle c_n \rangle \in \R^\N$.
    First we prove that reflexivity. Clearly, $\{n \in \N: a_n=a_n\}=\N \in \mc{F}^\co \subseteq \mc{F}$. Thus, $\langle a_n \rangle \equiv \langle a_n \rangle$. \\
    Symmetricity is trivial since $\{n \in \N: a_n=b_n\}=\{n \in \N: b_n=a_n\}$, if one of them is in $F$ then so is the other. \\
    Finally, we prove transitivity. Suppose $\la a_n \ra \equiv \la b_n \ra$ and $\la b_n \ra \equiv \la c_n \ra$ i.e. $\{n \in \N: a_n=b_n\}, \{n \in \N: b_n=c_n\} \in \mc{F}$. Clearly, $\{n \in \N: a_n=b_n=c_n\}=\{n \in \N: a_n=b_n\} \cap \{n \in \N: b_n=c_n\} \in \mc{F}$. Therefore, $\la a_n \ra \equiv \la c_n \ra$.
  \end{proof}
  \begin{exercise} (section 3.3, II)
    $\equiv$ is a congruence on the ring $\la \R^\N, \op, \od \ra$, which means that if $r \equiv r^\p$ and $s \equiv s^\p$, then $r \op s=r^\p \op s^\p$ and $r \od s=r^\p \od s^\p$.
  \end{exercise}
  \begin{proof}
    Suppose $r \equiv r^{\p}$ and $s \equiv s^{\p}$ i.e. $ \{n \in \N: r_n=r^\p_n \}, \{n \in \N: s_n=s_n^\p \} \in \mc{F}$. Thus, since $ \{n \in \N: r_n=r_n^\p, s_n=s_n^\p \}=\{n \in \N: r_n=r_n^\p \} \cap \{n \in \N: s_n=s_n^\p \} \in \mc{F}$, we have $\{n \in \N: r_n=r_n^\p, s_n=s_n^\p \} \subseteq \{n \in \N: r_n+s_n=r_n^\p+s_n^\p \} \in \mc{F}$. Similarly, $\{n \in \N: r_ns_n=r_n^\p s_n^\p \} \in \mc{F}$. Therefore, $r\op s \equiv r^\p \op s^\p$ and $r \od s \equiv r^\p \od s^\p$.
  \end{proof}
  \begin{exercise} (section 3.3, III)
    $\la 1, \frac{1}{2}, \frac{1}{3}, \cdots \ra \not \equiv \la 0, 0, 0, \cdots \ra$. 
  \end{exercise}
  \begin{proof}
    Let $\la r \ra=\la 1, \frac{1}{2}, \frac{1}{3}, \cdots \ra$. For the sake of simplicity, define $[[r \not =0]]=\{n \in \N:r_n \not =0\}$. Clearly, $[[r \not =0]] \subseteq \N$. Notice that for any $n \in \N$, we have $n \in [[r \not =0]]$. Thus, $[[r \not =0]]=\N$. So, $[[r \not =0]] \in \mc{F}^\co \subseteq \mc{F}$ but then it would mean $[[r=0]]=[[r \not=0]]^c \notin \mc{F}$. Therefore, $\la r_n \ra \not \equiv \la 0 \ra$.
  \end{proof}

  \begin{exercise}
    (section 3.5, I)
    $[[r=s]] \cap [[s=t]] \subseteq [[r=t]]$.
  \end{exercise}
  \begin{proof}
    Let $n \in [[r=s]] \cap [[s=t]]$. Then it follows that $r_n=s_n$ and $s_n=t_n$, and so $r_n=t_n$. Therefore, $n \in [[s=t]]$.
  \end{proof}

  \begin{exercise} (Section 3.5, II)
    $[[r=r^\p]] \cap [[s=s^\p]] \subseteq [[r \op s=r^\p \op s^\p]] \cap [[r \op s=r^\p \op s^\p]]$
  \end{exercise}
  \begin{proof}
    Let $n \in [[r=r^\p]] \cap [[s=s^\p]]$. Thus, $r_n=r_n^\p$ and $s_n=s_n^\p$, and so $r_n \op s_n=r_n^\p \op s_n^\p$ and $r_n \od s_n = r_n^\p \od s_n^\p$. Therefore, $n \in [[r \op s=r^\p \op s^\p]] \cap [[r \op s=r^\p \op s^\p]]$.
  \end{proof}
  \begin{exercise}
    (Section 3.5, III)
    $[[r=r^\p]] \cap [[s=s^\p]] \cap [[r<s]] \subseteq [[r^\p<s^\p]]$.
  \end{exercise}
  \begin{proof}
    Let $n \in [[r=r^\p]] \cap [[s=s^\p]] \cap [[r<s]]$. Thus, $r_n=r_n^\p, s_n=s_n^\p, r_n<s_n$ but then that means $r_n^\p<s_n^\p$, and so $ n \in [[r^\p<s^\p]]$.
  \end{proof}
  \begin{exercise} (Section 3.5, IV)
    If $r \equiv r^\p$ and $s \equiv s^\p$, then $[[r<s]] \in \mc{F}$ iff $[[r^\p<s^\p]] \in \mc{F}$.
  \end{exercise}
  \begin{proof}
    Suppose $r \equiv r^\p$ and $s \equiv s^\p$, that is to say, $\{n \in \N: r_n=r_n^\p\}, \{n \in \N: s_n=s_n^\p\} \in \mc{F}$. First assume $[[r<s]] \in \mc{F}$. Therefore, $\{n \in \N: r_n=r_n^\p\} \cap \{n \in \N: s_n=s_n^\p\} \cap \{n \in \N: r_n<s_n\} \subseteq \{n \in \N: r^\p<s^\p \} \in mc{F}$. Next assume $[[r^\p<s^p]] \in \mc{F}$. It follows $\{n \in \N: r_n=r_n^\p\} \cap \{n \in \N: s_n=s_n^\p\} \cap \{n \in \N: r_n^\p<s_n^\p\} \subseteq \{n \in \N: r<s\} \in \mc{F}$
  \end{proof}

  \begin{exercise}
    (Section 3.8, I)
    Use only general properties of ordered fields to deduce from the fact that $[\ep]$ is a positive infinitismal, the conclusion that $[\ep]^{-1}$ is greater than every real number.
  \end{exercise}
  \begin{proof}
    Notice that for any $r \in \R^+$, we have ${}^* r=[\la r,r,\cdots,\ra] \in {}^* \R$. Since $\ep<{}^* r$, by fields properties, we have $0<{}^* r^{-1}<\ep^{-1}$. Since $r$ is arbitrary positive real number, setting $r=r^{-1}$,we see that ${}^* r< \ep^{-1}$ for any $r \in \R^+$. 
  \end{proof}
  
  \begin{exercise} (Section 3.10, I)
    If $A$ is finite, show that ${}^*A=A$, and hence $A$ has non nonstandard members.
  \end{exercise}
  \begin{proof}
    Let $A=\{a_1,\cdots, a_n\}$. Consider some $[r] \in {}^* A$. If we could prove that $r \equiv t$ for some constant sequence $t \in A$, we would be done. So we set that as our goal. Notice that since $[r] \in {}^* A$, we have $\{ n \in \N: r_n \in A\}= \{n \in \N: r_n=a_1 \lor r_n=a_2 \lor \cdots r_n=a_n\}=\{n \in \N: r_n=a_1\} \cup \cdots \cup \{n \in \N:r_n=a_n\} \in \mc{F}$. But since $\mc{F}$ is ultrafilter, only one of such set is in $\mc{F}$. Therefore, $\{n \in \N: r_n=a_k\} \in \mc{F}$ for some $k$ such that $1 \leq k \leq n$. Hence, $r \equiv a_k$.
  \end{proof}

  \begin{exercise}
    (Section 3.10, II) 
    Prove: \\
    (a) $A \subseteq B$ iff ${}^* A \subseteq {}^* B$. \\
    (b) $A=B$ iff ${}^* A = {}^* B$.
  \end{exercise}
  \begin{proof} $ $ \\
    (a) First we prove the forward implication. Suppose $A \subseteq B$. Consider $[r] \in {}^* A$. Therefore, we have $[[r \in A]] \in \mc{F}$, but since $[[r \in A]] \subseteq [[r \in B]]$, we have $[[r \in B]]$ and so $[r] \in {}^* B$. \\
    We prove the converse implication. Suppose ${}^* A \subseteq {}^* B$. Consider some $r \in A$. Then we have $[\mb{r}] \in {}^* A$, and so $[\mb{r}] \in {}^*B$. However, since $[{\mb{r}}] \in B$, we have $[[r \in B]] \in \mc{F}$ which means $r \in B$. \\

    (b) Trivially follows from (a).
  \end{proof}

  \begin{exercise}
    (Section 3.10, III) \\
    Prove: \\
    (a) ${}^* (A \cup B) = {}^* A \cup {}^* B$, \\
    (b) ${}^* (A \cap B)= {}^* A \cap {}^* B$, \\
    (c) $\hyp (A-B)=\hyp A - \hyp B$, \\
    (d) $\hyp \emptyset =\emptyset$.
  \end{exercise}
  \begin{proof} $ $ \\
    (a) First we prove the foward implication. Since $A \subset A \cup B$, applying (2), we have ${}^* A \subseteq {}^* (A \cup B)$. Similarly, we have ${}^* B \subseteq {}^* (A \cup B)$, and so ${}^* A \cup {}^* B \subseteq {}^* (A \cup B)$. \\
    We prove the converse implication. Let $[r] \in {}^* A \cup {}^* B$. Then we have following cases; \\
    \textbf{case-1.} $[r] \in {}^* A$. Thus, $[[r \in A]] \in mc{F}$, and since $[[r \in A]] \subseteq [[r \in A \cup B]]$, we have $[[r \in A \cup B]] \in \mc{F}$ but that means $[r] \in {}^* A \cup {}^* B$. \\
    \textbf{case-2.} $[r] \in {}^* B$. The proof is analogous to \textbf{case-1}. \\

    (b) First we prove the forward implication. Since $A \cap B \subseteq A$, applying (2), we have ${}^* (A \cap B) \subseteq {}^* A$. Similarly we have $\hyp (A \cap B) \subseteq \hyp B$, and so $\hyp (A \cap B) \subseteq \hyp A \cap \hyp B$. \\
    We prove the converse implication. Consider some $[r] \in \hyp A \cap \hyp B$. It means that $[r] \in \hyp A$ and $[r] \in \hyp B$, thus $[[r \in A]], [[r \in B]] \in \mc{F}$. Therefore, $[[r \in A \cap B]]=[[r \in A]] \cap [[r \in B]] \in \mc{F}$, and so $[r] \in \hyp (A \cap B)$.  \\

    (c) First we prove the foward implication. Let $[r] \in \hyp (A \setminus B)$. Then we have $[[r \in A]] \cap [[r \notin B]]=[[r \in A \setminus B]] \in \mc{F}$. Thus, $[[r \in A]], [[r \notin B]] \in \mc{F}$. Hence, $[r] \in \hyp A$ and $[r] \notin \hyp B$, and so $[r] \in \hyp A \setminus \hyp B$. \\
    We prove the converse implication. Let $[r] \in \hyp A \setminus \hyp B$ i.e. $[r] \in \hyp A$ and $[r] \notin \hyp B$. Then we have $[[r \in A]] \in \mc{F}$ and $[[r \notin B]] \in \mc{F}$. Thus, $[[r \in A \setminus B]]=[[r \in A]] \cap [[r \notin B]] \in \mc{F}$. Therefore, $r \in \hyp (A \setminus B)$. \\

    (d) Clearly, $\hyp \emptyset =\{ [r] \in \hyp \R: [[r \in \emptyset]] \in \mc{F}\}=\emptyset$. 
  \end{proof}

  \begin{exercise}
    (Section 3.10, IV)
    Is it true that $\hyp (\bigcup_{n=1}^\infty A_n)=\bigcup_{n=1}^\infty \hyp A_n$?
  \end{exercise}
  \begin{proof}
    No. Define $A_n=\{n\}$ for any $n \in \N$. Notice that since $A_n$ is finite, using (1), we have $\hyp A_n=A_n=\{n\}$. Since $[[\omega \in \bigcup_{n=1}^\infty A_n]]=\N \in \mc{F}$, we have $\omega \in \hyp (\bigcup_{n=1}^\infty A_n)$. However, $[[\omega \in A_n]]=\{n\} \notin \mc{F}$, thus $\omega \notin \hyp A_n$ for any $n \in \N$. This mean $\omega \notin \bigcup_{n=1}^\infty \hyp A_n$.
  \end{proof}

  \begin{exercise}
    (Section 3.10, V)
    Show that if $A \subseteq \R$, then $\hyp A \cap \R =A$.
  \end{exercise}
  \begin{proof}
    Suppose $A \subseteq \R$. Let $[r] \in \hyp A \cap \R$. Since $\la r \ra$ is a constant sequence and $[r] \in \hyp A$, it follows $[r]=\la r \ra \in A$. Thus, $\hyp A \cap \R \subseteq A$. This means that $\hyp A \cap \R$ contains only the constant sequences. Let $\la r \ra \in A$. Then clearly $[r] \in \hyp A \cap \R$.
  \end{proof}

  \begin{exercise}
    For $a,b \in \R$, let $[a,b]$ be the closed interval $\{x \in \R: a \leq x \leq n\}$. Prove that $\hyp [a,b]=\{x \in \hyp \R: a \leq x \leq b\}$.
  \end{exercise}
  \begin{proof}
    We first prove the forward inclusion. Let $[r] \in \hyp [a,b]$. Then we have $\{n \in \N: a \leq r_n \leq b\}=[[r \in [a,b]]] \in \mc{F}$ but that means $[r] \in \{x \in \hyp \R: a \leq x \leq b\}$. We prove the converse inclusion. Let $[r] \in \{x \in \hyp \R: a \leq x \leq b\}$. It follows $[[r \in [a,b]]]=\{n \in \N: a \leq r_n \leq b\} \in mc{F}$. Therefore, $[r] \in \{x \in \R: a \leq x \leq n\}$.
  \end{proof}

  \begin{exercise}
    (Section 3.10, VII) 
    $\hyp \Z$ is a subring of $\hyp \R$.
  \end{exercise}
  \begin{proof}
    Clearly, $\hyp \Z \not = \emptyset$. Consider some $[r], [s] \in \hyp \Z$. Then we have $[[r \in \Z]], [[s \in \Z]] \in \mc{F}$. Therefore, since $[[r \in \Z]] \cap [[s \in \Z]] \subseteq [[r+s \in \Z]], [[rs \in \Z]]$, we have $[[r+s \in \Z]], [[rs \in \Z]] \in \mc{F}$. Hence, $[r+s], [rs] \in \hyp \Z$.
  \end{proof}

  \begin{exercise}
    (Section 3.10, VIII)
    If $\R^+=\{x \in \R: x>0\}$, show that $\hyp (\R^+)=\{x \in \hyp \R^+:x>0\}$, i.e., $\hyp (R^+)=(\hyp \R)^+$.
  \end{exercise}
  \begin{proof}
    First we prove the forward inclusion. Let $[r] \in \hyp (R^+)$. It means that $\{n \in \N: r_n>0\}=[[r \in R^+]] \in \mc{F}$ which implies $[r] \in (\hyp \R)^+$. Next we prove the converse inclusion. Let $[r] \in (\hyp \R)^+$. Then we have $\{n \in \N: r_n>0\}=[[r>0]]=[[r \in \R^+]] \in \mc{F}$ from which it follows $[r] \in \hyp(\R^+)$.
  \end{proof}

  \begin{exercise}
    (Section 3.12, I)
    Show that $\hyp f$ agrees with $f$ on $\R$: if $r \in \R$, then $\hyp f(r)=f(r)$.
  \end{exercise}
  \begin{proof}
    Let $r \in \R$. Notice that $r$ can be indetified with the constant sequence $\mb{r} \in \hyp R$. Then we have $\hyp f([\mb{r}])=[f(\mb{r})]$ which is isomorphic to $f(r)$.
  \end{proof}
  \begin{exercise}
    (Section 3.12, II)
    If $f$ is injective, so is $\hyp f$. What about surjectivity?
  \end{exercise}
  \begin{proof}
    Suppose $f$ is injective. Consider some $[r], [s] \in \hyp \R$ such that $\hyp f([r])=\hyp f([s])$, that is to say $[f \circ r]=[f \circ s]$. Since $f$ is injective, we have $[[f \circ r=f \circ s]] \subseteq [[r =s]]$ but then, since $[[f \circ r=f \circ s]] \in \mc{F}$, it follows $[[r=s]] \in \mc{F}$. Therefore, $[r]=[s]$. \\

    Yes, surjecitivity is preserved. Suppose $f$ is surjective. Consider some $[s] \in \hyp \R$. Our goal is to prove that there is some $[r] \in \hyp \R$ such that $\hyp f([r])=[s]$. Define sequenece $(r_n)$ such that, for each $s_n$, $f(r_n)=s_n$. We know such a $r_n$ exists for each $s_n$ since $f$ is surjective. We claim that $[r] \in \hyp \R$ the element we looking for. To prove this claim, we need to show $[f \circ r]=f([r])=[s]$, so we set that as our goal. Clearly, $[[f \circ r = s]]=\{n \in \N: f(r_n)=s_n\}=\N \in \mc{F}$. Therefore, $[f \circ r]=f[r] = [s]$. 
  \end{proof}

  \begin{exercise}
    (Section 3.12, III)
     For $x \in \hyp \R$, let $$|x| = \begin{cases} x, \text{ if } x>0 \\ 0, \text{ if } x=0 \\ -x \text{ if } x<0 \end{cases}$$ be the usal definition of absolute value function. Show that this extends the definition of $|.|$ on $\R$: $|[r]|=[ \la |r_1|, |r_2|,\cdots \ra]=[|r_n|]$.
  \end{exercise}
  \begin{proof}
    We have the following cases; \\
    \textbf{Case-1.} Suppose $[r]>0$. Then $[[r>0]] \in \mc{F}$. Since $[[r>0]] \subseteq [[ [r]=[|r|]]] \in \mc{F}$, we have $|[r]|=[r]=[|r_n|]$. \\
    \textbf{Case-2.} Suppose $[r]=0$. That is to say $[[r=0]] \in \mc{F}$. Since $[[r=0]] \subseteq [[0=|r|]] \in \mc{F}$, we have $|[r]|=0=[|r|]$. \\
    \textbf{Case-3.} Suppose $[r]<0$. Then $| [r]|=-[r]=[-r]=[|r|]$.
  \end{proof}

  \begin{exercise}
    (Section 3.12, IV)
    Let $\chi_A$ be the characteristic function of a set $A \subseteq \R$. Show that $\hyp (\chi_A)=\chi_{\hyp A}$.
  \end{exercise}
  \begin{proof}
    Let $[r] \in \hyp \R$. Consider the expression $\hyp (\chi_A)[r]$, we have the following cases; \\
    \textbf{Case-1.} Suppose $[r] \in \hyp A$. Notice that $\hyp (\chi_A)[r]=[\chi_A \circ r]=[\chi_A(r_n)]$ but then, since $[[r \in A]] \in \mc{F}$ and $[[r \in A]] \subseteq [[\chi_A \circ r=1]]$, we have $[[\chi_A \circ r=1]] \in \mc{F}$. Therefore, $[\chi_A \circ r]=\chi_A [r]=1$. \\
    \textbf{Case-2.} Suppose $[r] \notin \hyp A$. Then we have $[[r \notin A]]=[[r \in A]]^c \in \mc{F}$. Clearly, $[[r \notin A]] \subseteq [[\chi_A \circ r=0]]$. Thus, $[[\chi_A \circ r=0]] \in \mc{F}$ and so $[\chi_A \circ r]=\chi_A [r]=0$.
  \end{proof}
  \begin{exercise}
    (Section 3.12, V)
    Show how to define $\hyp f$ when $f$ is a function of more than one arguement.
  \end{exercise}
  \begin{proof}
    Define $\hyp f([r^1],\cdots,[r^n])=[f(r^1_1, \cdots, r^n_1),f(r^1_2,\cdots, r^n_2), \cdots]$. We prove that it's well defined. Clearly, $[[r^1=r^{1^\p}]] \cap \cdots [[r^n=r^{n^\p}]] \subseteq [[f \circ (r^1,\cdots, r^n)=f \circ (r^{1^\p}, \cdots, r^{n^\p})]]$. Therefore, $r^1 \equiv r^{1^\p}, \cdots, r^n \equiv r^{n^\p}$ implies $f \circ (r^1,\cdots, r^n) \equiv f \circ (r^{1^\p}, \cdots, r^{n^\p}$.
  \end{proof}

  \begin{exercise}
    (Section 3.15, I)
    If $A_1,\cdots, A_k$ are subsets of $\R$, put $P=A_1\times \cdots \times A_k$ and apply the definition of $\hyp P$ to show that $$ \hyp (A_1 \times \cdots \times A_k)=\hyp A_1 \times \cdots \times \hyp A_k.$$
  \end{exercise}
  \begin{proof}
    For $([r^1], [r^2], \cdots, [r^k]) \in \hyp P$, we must have $[[(r^1, r^2, \cdots, r^k) \in P]] \in \mc{F}$. Clearly, $[[(r^1, r^2, \cdots, r^k) \in P]] \subseteq [[r^n \in A_n]]$, thus $[[r^n \in A_n]]$ for any $n$ such that $1 \leq n \leq k$. This means that $[r^n] \in A^n$ for all such $n$. Hence, $([r^1], \cdots, [r^n]) \in \hyp A_1 \times \cdots \hyp A_n$. From this, it follows that $\hyp (\R^k)=(\hyp \R)^k$.
  \end{proof}

  \begin{exercise}
    (Section 3.15, II)
    Let $\dom P$ denote the domain of a binary relation. If $P \subseteq \R^2$, show that $\hyp (\dom P)= \dom \hyp P$.
  \end{exercise}
  \begin{proof}
    First we prove the forward inclusion. Let $[r] \in \hyp (\dom P)$. Then we have $\{n \in \N: r_n \in \dom P\}=[[r \in \dom P]] \in \mc{F}$. $$\text{ Define sequence } s_n = \begin{cases} s \text{ such that } (r_n, s) \in P, \text{ if } r_n \in \dom P \\ 0, \text{ if } r_n \notin \dom P \end{cases}$$ Then clearly, $[[(r,s) \in P]]=[[r \in \dom P]] \in \mc{F}$, but that means $([r], [s]) \in \hyp P$, and so $[r] \in \dom \hyp P$. \\
    Now we prove the converse inclusion. Let $[r] \in \dom \hyp P$. It follows that there exists $[s] \in \hyp \R$ such that $([r], [s]) \in \hyp P$, but that means $[[r \in \dom P]]=[[(r,s) \in P]] \in \mc{F}$. Hence, $[r] \in \hyp (\dom P)$.
  \end{proof}

\chapter{The Transfer Principle}

  \begin{exercise}
    
  \end{exercise}



\end{document}

